src/StackMachComp.v
@@ -362,8 +362,11 @@ Section Preservation.
   Theorem fsim :
     Semantics.forward_simulation (A.semantics prog) (B.semantics tprog).
   Proof.
-    eapply Semantics.forward_simulation_step with (match_states := I).
-    - inversion 1. (* TODO - replace with callstate matching *)
+    eapply Semantics.forward_simulation_step with
+        (match_states := I)
+        (match_values := @eq value).
+    - simpl. intros. eexists. split. 2: econstructor.
+      on >B.is_callstate, invc. repeat i_ctor.
     - intros0 II Afinal. invc Afinal; invc II. eexists; split.
       constructor. reflexivity.
     - intros0 Astep. intros0 II.
